Support for arrays has been added, e.g. the following program
  temp := a[i];
  a[i] := a[j];
  a[j] := temp

is translated into
  
  |- Swap (i,j,temp,a) =
       let temp = a ' i in
       let a = a |+ (i,j) in
       let a = a |+ (j,temp) in
         (i,j,temp,a)

and the automatically proved theorem is:

  |- SEP_SPEC 
       (ARRAY "a" a * VAR "i" i * VAR "j" j * VAR "temp" temp)
       (Seq (Assign "temp" (Arr "a" (Var "i")))
            (Seq (ArrayAssign "a" (Var "i") (Var "j"))
                 (ArrayAssign "a" (Var "j") (Var "temp"))))
       (let (i,j,temp,a) = Swap (i,j,temp,a) in
         (ARRAY "a" a * VAR "i" i * VAR "j" j * VAR "temp" temp))

examples/opsem_extract/opsem_translatorLib.sml
@@ -11,6 +11,7 @@ val cdr = snd o dest_comb
 
 fun mk_star (tm1,tm2) = (fst o dest_eq o concl o ISPECL [tm1,tm2]) STAR_COMM
 fun mk_VAR (tm1,tm2) = (fst o dest_eq o concl o ISPECL [tm1,tm2]) VAR_def
+fun mk_ARRAY (tm1,tm2) = (fst o dest_eq o concl o ISPECL [tm1,tm2]) ARRAY_def
 fun mk_SEP_SPEC (pre,prog,post) = (fst o dest_eq o concl o ISPECL [pre,prog,post]) SEP_SPEC_def
 
 fun list_mk_star [] = ``emp:state->bool``
@@ -19,6 +20,8 @@ fun list_mk_star [] = ``emp:state->bool``
 
 fun is_emp tm = fst (dest_const tm) = "emp" handle HOL_ERR _ => false;
 fun is_VAR tm = repeat car tm = ``VAR``
+fun is_ARRAY tm = repeat car tm = ``ARRAY``
+fun is_VAR_or_ARRAY x = (is_VAR x orelse is_ARRAY x) 
 
 fun dest_star tm = let
   val (x,z) = dest_comb tm
@@ -37,27 +40,32 @@ val POST_CONV = RAND_CONV
 fun SORT_VAR_CONV tm = let
   val xs = list_dest_star tm
   val get_varname = fromHOLstring o cdr o car
-  val ys = sort (fn x => fn y => get_varname x < get_varname y) (filter is_VAR xs)
-  val tm2 = list_mk_star (ys @ filter (not o is_VAR) xs)
+  val ys = sort (fn x => fn y => get_varname x < get_varname y) (filter is_VAR_or_ARRAY xs)
+  val tm2 = list_mk_star (ys @ filter (not o is_VAR_or_ARRAY) xs)
   in prove(mk_eq(tm,tm2),SIMP_TAC bool_ss [AC STAR_ASSOC STAR_COMM,emp_STAR]) end
   handle HOL_ERR _ => ALL_CONV tm;
 
 val SPEC_SORT_VAR_RULE = CONV_RULE 
   (REWRITE_CONV [emp_STAR] THENC PRE_CONV SORT_VAR_CONV THENC POST_CONV SORT_VAR_CONV); 
 
-fun EVAL_beval_neval exp = let
+fun EVAL_beval_neval_aeval exp = let
   val tm = subst [``e:nexp``|->exp] ``neval e s`` 
            handle HOL_ERR _ => subst [``e:bexp``|->exp] ``beval e s``
-  val e = (snd o dest_eq o concl o SIMP_CONV bool_ss [neval_def,beval_def]) tm
-  val vs = find_terms (can (match_term ``s:state ' x``)) e
-  in subst (map (fn v => v |-> mk_var(fromHOLstring (cdr v),type_of v)) vs) e end
+           handle HOL_ERR _ => subst [``e:aexp``|->exp] ``aeval e s``
+  val e = (snd o dest_eq o concl o SIMP_CONV bool_ss [neval_def,aeval_def,beval_def]) tm
+  val vs = find_terms (can (match_term ``ScalarOf (s:state ' x)``)) e
+  val e = subst (map (fn v => v |-> mk_var(fromHOLstring (cdr (cdr v)),type_of v)) vs) e
+  val vs = find_terms (can (match_term ``ArrayOf (s:state ' x)``)) e
+  val e = subst (map (fn v => v |-> mk_var(fromHOLstring (cdr (cdr v)),type_of v)) vs) e
+  in e end
 
-fun SPEC_FILL_AND_SORT th1 th2 vs = let
+fun SPEC_FILL_AND_SORT th1 th2 vs ws = let
   val vs = map mk_VAR (map (fn v => (fromMLstring v,mk_var(v,``:int``))) vs)    
+  val ws = map mk_ARRAY (map (fn v => (fromMLstring v,mk_var(v,``:int|->int``))) ws)    
   val p1 = (list_dest_star o cdr o car o car o concl) th1
   val p2 = (list_dest_star o cdr o car o car o concl) th2
-  val add_to1 = filter (fn x => not (mem x p1)) (all_distinct (p2 @ vs))
-  val add_to2 = filter (fn x => not (mem x p2)) (all_distinct (p1 @ vs))
+  val add_to1 = filter (fn x => not (mem x p1)) (all_distinct (p2 @ vs @ ws))
+  val add_to2 = filter (fn x => not (mem x p2)) (all_distinct (p1 @ vs @ ws))
   fun apply_frame th = MATCH_MP SEP_SPEC_FRAME th handle HOL_ERR _ =>
                        MATCH_MP SEP_TOTAL_SPEC_FRAME th
   val th1 = SPEC (list_mk_star add_to1) (apply_frame th1)
@@ -80,26 +88,63 @@ fun FORCE_PBETA_CONV tm = let
     handle e => ALL_CONV
   in (RAND_CONV (get_conv vs) THENC PairRules.PBETA_CONV) tm end;
 
+fun get_scalar_and_array_varnames tm = let
+  val vs = map fromHOLstring (find_strings tm)
+  val scalars = map (fromHOLstring o cdr) (find_terms (can (match_term ``Var v``)) tm)
+  val a = (find_terms (can (match_term ``Assign v``)) tm)
+  val scalars = scalars @ (map (fromHOLstring o cdr) a)
+  val vs = all_distinct (filter (fn s => not (mem s scalars)) vs)
+  val scalars = all_distinct scalars
+  in (scalars,vs) end;
+
+fun get_VAR_and_ARRAY tm v = let
+  val (scalars,vs) = get_scalar_and_array_varnames tm
+  val vs = filter (fn w => not (w = v)) vs
+  val scalars = filter (fn w => not (w = v)) scalars
+  val vs = map mk_ARRAY (map (fn v => (fromMLstring v,mk_var(v,``:int |-> int``))) vs)    
+  val scalars = map mk_VAR (map (fn v => (fromMLstring v,mk_var(v,``:int``))) scalars)    
+  in scalars @ vs end;
+
+fun PROVE_SEP_EXP th = 
+  MATCH_MP th (prove((fst o dest_imp o concl) th,
+    SIMP_TAC std_ss [SEP_EXP_def,SEP_GUARD_def,pairTheory.FORALL_PROD,GSYM STAR_ASSOC,
+      GEN_VAR_STAR,aeval_def,beval_def,neval_def,DOMSUB_FAPPLY_THM,VAR_def,
+      ScalarOf_def,ArrayOf_def,ARRAY_def]
+    THEN CONV_TAC (DEPTH_CONV stringLib.string_EQ_CONV)
+    THEN SIMP_TAC std_ss [ScalarOf_def,ArrayOf_def]));
+
 fun MK_SEP_SPEC_ASSIGN tm total = let
   val v = (fromHOLstring o cdr o car) tm
-  val vs = map fromHOLstring (find_strings tm)
-  val vs = all_distinct (filter (fn s => not (s = v)) vs)
-  val vs = map mk_VAR (map (fn v => (fromMLstring v,mk_var(v,``:int``))) vs)    
+  val vs = get_VAR_and_ARRAY tm v
   val p = list_mk_star vs   
   val z = list_mk_pair(free_vars p) handle e => genvar(``:int``)
-  val rhs = EVAL_beval_neval (cdr tm)
+  val rhs = EVAL_beval_neval_aeval (cdr tm)
   val n = mk_pabs(mk_pair(mk_var(v,``:int``),z),rhs) 
   val th = ISPEC (mk_pabs (z, p)) SEP_SPEC_ASSIGN
   val th = SPECL [fromMLstring v,mk_var(v,``:int``),z,cdr tm,n] th
-  val goal = (fst o dest_imp o concl) th
-  val th = MATCH_MP th (prove(goal,
-    SIMP_TAC std_ss [SEP_EXP_def,pairTheory.FORALL_PROD,GSYM STAR_ASSOC,VAR_STAR,
-      beval_def,neval_def,DOMSUB_FAPPLY_THM]
-    THEN CONV_TAC (DEPTH_CONV stringLib.string_EQ_CONV)
-    THEN SIMP_TAC std_ss []))
+  val th = PROVE_SEP_EXP th
   val th = SPEC_SORT_VAR_RULE (SIMP_RULE std_ss [] th)
   val th = if total then REWRITE_RULE [SEP_TOTAL_ASSIGN_THM] th else th
   in (th,(mk_var(v,``:int``),rhs)) end;
+
+fun MK_SEP_SPEC_ARRAY_ASSIGN tm total = let
+  val v = (fromHOLstring o cdr o car o car) tm
+  val vs = get_VAR_and_ARRAY tm v
+  val p = list_mk_star vs   
+  val z = list_mk_pair(free_vars p) handle e => genvar(``:int |-> int``)
+  val rhs2 = EVAL_beval_neval_aeval (cdr tm)
+  val rhs1 = EVAL_beval_neval_aeval (cdr (car tm))
+  val n2 = mk_pabs(mk_pair(mk_var(v,``:int |-> int``),z),rhs2) 
+  val n1 = mk_pabs(mk_pair(mk_var(v,``:int |-> int``),z),rhs1) 
+  val th = ISPEC (mk_pabs (z, p)) SEP_SPEC_ARRAY_ASSIGN
+  val th = SPECL [fromMLstring v,mk_var(v,``:int|->int``),z,cdr (car tm), cdr tm,n1,n2] th
+  val th = PROVE_SEP_EXP th
+  val th = PROVE_SEP_EXP th
+  val rhs = (cdr o cdr o car o cdr o concl) th
+  val rhs = (cdr o concl o SIMP_CONV std_ss []) rhs
+  val th = SPEC_SORT_VAR_RULE (SIMP_RULE std_ss [] th)
+  val th = if total then REWRITE_RULE [SEP_TOTAL_ARRAY_ASSIGN_THM] th else th
+  in (th,(mk_var(v,``:int|->int``),rhs)) end;
 
 fun FORCE_DISCH th = let
   val th = PURE_REWRITE_RULE [GSYM CONJ_ASSOC,AND_IMP_INTRO] (DISCH_ALL th)
@@ -108,7 +153,7 @@ fun FORCE_DISCH th = let
 fun is_total th = repeat car (concl th) = ``SEP_TOTAL_SPEC``;
 
 fun MK_SEP_SPEC_SEQ th1 th2 = let
-  val (th1,th2) = SPEC_FILL_AND_SORT th1 th2 []
+  val (th1,th2) = SPEC_FILL_AND_SORT th1 th2 [] []
   val (i,t) = match_term ((cdr o car o car o concl) th2) ((cdr o concl) th1)
   val th2 = INST i (INST_TYPE t th2)
   in if not (is_total th1) then MATCH_MP SEP_SPEC_SEQ (CONJ th1 th2) else 
@@ -118,31 +163,34 @@ fun MK_SEP_SPEC_SEQ th1 th2 = let
 
 fun VARS_UNBETA_CONV tm = let
   val vs = filter is_VAR (list_dest_star tm)
-  val x = list_mk_pair (map cdr vs)    
-  val xs = map (fromHOLstring o cdr o car) vs
-  val ys = map (fn v => mk_VAR(fromMLstring v,mk_var(v,``:int``))) xs
-  val tm1 = list_mk_star (ys @ filter (not o is_VAR) (list_dest_star tm))
-  val p = list_mk_pair (map(fn v => mk_var(v,``:int``)) xs)
+  val ws = filter is_ARRAY (list_dest_star tm)
+  val x = list_mk_pair (map cdr (vs @ ws))    
+  val vs = map (fromHOLstring o cdr o car) vs
+  val ws = map (fromHOLstring o cdr o car) ws
+  val vs' = map (fn v => mk_VAR(fromMLstring v,mk_var(v,``:int``))) vs
+  val ws' = map (fn v => mk_ARRAY(fromMLstring v,mk_var(v,``:int|->int``))) ws
+  val tm1 = list_mk_star (vs' @ ws' @ filter (not o is_VAR_or_ARRAY) (list_dest_star tm))
+  val tm1 = (cdr o concl o SORT_VAR_CONV) tm1 
+  val p = list_mk_pair (map(fn v => mk_var(v,``:int``)) vs @ 
+                        map(fn v => mk_var(v,``:int|->int``)) ws)
   val tm2 = mk_comb(mk_pabs(p,tm1),x)
   val goal = mk_eq(tm,tm2)
   in prove(goal,SIMP_TAC std_ss [AC STAR_ASSOC STAR_COMM, emp_STAR]) end;
 
 fun MK_SEP_GUARD h th1 = let
   val (x,y) = (dest_comb o cdr o car o car o concl) th1
-  val g = mk_pabs(y,EVAL_beval_neval h)
+  val g = mk_pabs(y,EVAL_beval_neval_aeval h)
   val tm = repeat car (inst [``:'a``|->type_of y] ``SEP_GUARD p (g:'a->bool) h``)
   val goal = mk_comb(mk_comb(mk_comb(tm,x),g),h)
-  val th = prove(goal,
-    SIMP_TAC std_ss [SEP_GUARD_def,pairTheory.FORALL_PROD,GSYM STAR_ASSOC,VAR_STAR,
-      beval_def,neval_def,DOMSUB_FAPPLY_THM]
-    THEN CONV_TAC (DEPTH_CONV stringLib.string_EQ_CONV)
-    THEN SIMP_TAC std_ss [])
+  val lemma = prove(``!b. b ==> b:bool``,REPEAT STRIP_TAC THEN ASM_REWRITE_TAC [])
+    val th = SPEC goal lemma
+  val th = PROVE_SEP_EXP th
   in (g,th) end;
 
 fun MK_SEP_SPEC_COND th1 th2 h = let
   val total = is_total th1
-  val vs = map fromHOLstring (find_strings h)
-  val (th1,th2) = SPEC_FILL_AND_SORT th1 th2 vs
+  val (vs,ws) = get_scalar_and_array_varnames h
+  val (th1,th2) = SPEC_FILL_AND_SORT th1 th2 vs ws
   val th1 = CONV_RULE (PRE_CONV VARS_UNBETA_CONV THENC POST_CONV VARS_UNBETA_CONV) th1
   val th2 = CONV_RULE (PRE_CONV VARS_UNBETA_CONV THENC POST_CONV VARS_UNBETA_CONV) th2
   val (g,th) = MK_SEP_GUARD h th1
@@ -153,8 +201,8 @@ fun MK_SEP_SPEC_COND th1 th2 h = let
 
 fun MK_SEP_SPEC_WHILE th1 h = let
   val total = is_total th1
-  val vs = map fromHOLstring (find_strings h)
-  val th1 = fst (SPEC_FILL_AND_SORT th1 SEP_SPEC_SKIP vs)
+  val (vs,ws) = get_scalar_and_array_varnames h
+  val th1 = fst (SPEC_FILL_AND_SORT th1 SEP_SPEC_SKIP vs ws)
   val th1 = CONV_RULE (PRE_CONV VARS_UNBETA_CONV THENC POST_CONV VARS_UNBETA_CONV) th1
   val (g,th) = MK_SEP_GUARD h th1
   val p = (cdr o cdr o car o car o concl) th1
@@ -190,28 +238,53 @@ fun mk_lets [] p = p
   if fst (last lets) = p then list_mk_anylet(map (fn x => [x]) (butlast lets), snd (last lets))
                          else list_mk_anylet(map (fn x => [x]) lets, p)
 
-fun SPEC_FOR_SEQ instr_tm index name rw_th total = let
-  val func_name = if index = 0 then name else name ^ "_" ^ int_to_string index 
+(*
+val total = true
+val name = "hoo"
+val index = 0
+val instr_tm = ``(While (Not (Equal (Var "n") (Const 0)))
+                   (Assign "n" (Sub (Var "n") (Const 2))))``
+
+val instr_tm = ``(While (Not (Equal (Var "n") (Const 0)))
+                   (Seq (Assign "a" (Plus (Var "a") (Const 1)))
+                        (Assign "n" (Sub (Var "n") (Const 2)))))``
+*)
+
+fun SPEC_FOR_SEQ instr_tm index name total = let
+  val func_name = if index = 0 then name else name ^ int_to_string index 
   in if repeat car instr_tm = ``Skip`` then 
-    (if total then SEP_TOTAL_SPEC_SKIP else SEP_SPEC_SKIP,[],index,rw_th) 
+    (if total then SEP_TOTAL_SPEC_SKIP else SEP_SPEC_SKIP,[],index,TRUTH,TRUTH) 
   else if repeat car instr_tm = ``Assign`` then let
     val (th,(lhs,rhs)) = MK_SEP_SPEC_ASSIGN instr_tm total
-    in (th,[(lhs,rhs)],index,rw_th) end
+    in (th,[(lhs,rhs)],index,TRUTH,TRUTH) end
+  else if repeat car instr_tm = ``ArrayAssign`` then let
+    val (th,(lhs,rhs)) = MK_SEP_SPEC_ARRAY_ASSIGN instr_tm total
+    in (th,[(lhs,rhs)],index,TRUTH,TRUTH) end
   else if repeat car instr_tm = ``Seq`` then let
-    val (th1,lets1,i1,rw_th) = SPEC_FOR_SEQ ((cdr o car) instr_tm) index name rw_th total
-    val (th2,lets2,i2,rw_th) = SPEC_FOR_SEQ (cdr instr_tm) i1 name rw_th total
+    val (th1,lets1,i1,rw_th1,rw_pre1) = SPEC_FOR_SEQ ((cdr o car) instr_tm) index name total
+    val (th2,lets2,i2,rw_th2,rw_pre2) = SPEC_FOR_SEQ (cdr instr_tm) i1 name total
     val th = MK_SEP_SPEC_SEQ th1 th2
-    in (th,lets1@lets2,i2,rw_th) end
+    val f = fst o dest_imp o concl o FORCE_DISCH 
+    val tm2 = f th2
+    val tm2 = if tm2 = T then T else mk_lets lets1 tm2
+    val goal = mk_eq(f th, mk_conj(f th1,tm2))    
+    val lemma = prove(goal,SIMP_TAC std_ss [LET_DEF]    
+               THEN CONV_TAC (DEPTH_CONV FORCE_PBETA_CONV)
+               THEN REPEAT STRIP_TAC THEN EQ_TAC THEN REPEAT STRIP_TAC
+               THEN ASM_SIMP_TAC std_ss [LET_DEF])
+    val th = CONV_RULE (RATOR_CONV (RAND_CONV (fn tm => lemma))) (FORCE_DISCH th)
+    val th = UNDISCH_ALL (REWRITE_RULE [] th)
+    val rw_th = CONJ rw_th1 rw_th2
+    val rw_pre = CONJ rw_pre1 rw_pre2
+    in (th,lets1@lets2,i2,rw_th,rw_pre) end
   else if repeat car instr_tm = ``Cond`` then let
-    val (th1,lets1,i1,rw_th) = SPEC_FOR_SEQ ((cdr o car) instr_tm) (index+1) name rw_th total
-    val (th2,lets2,i2,rw_th) = SPEC_FOR_SEQ (cdr instr_tm) i1 name rw_th total
-
+    val (th1,lets1,i1,rw_th1,rw_pre1) = SPEC_FOR_SEQ ((cdr o car) instr_tm) (index+1) name total
+    val (th2,lets2,i2,rw_th2,rw_pre2) = SPEC_FOR_SEQ (cdr instr_tm) i1 name total
     val th = MK_SEP_SPEC_COND th1 th2 ((cdr o car o car) instr_tm)
     val tm = (cdr o cdr o concl) th
     val (g_tm,t1,t2) = dest_cond tm
     val g = (cdr o concl o SIMP_CONV std_ss []) g_tm
     val t0 = cdr g_tm
-
     val t4 = if index = 0 then t0 else list_mk_pair (find_modified t0 t1 t2)
     val l1 = mk_lets lets1 t4
     val l2 = mk_lets lets2 t4
@@ -237,11 +310,17 @@ fun SPEC_FOR_SEQ instr_tm index name rw_th total = let
     val th = SIMP_RULE std_ss [] th
     val th = FORCE_DISCH th
     val th = REWRITE_RULE [] (CONV_RULE ((RATOR_CONV o RAND_CONV) (SIMP_CONV std_ss [])) th)
+    val (th,def_pre) = if not (is_imp (concl th)) then (th,TRUTH) else let
+      val f_pre = mk_var(func_name^"_pre",mk_type("fun",[type_of (cdr g_tm),``:bool``]))
+      val def_pre = Define [ANTIQUOTE (mk_eq(mk_comb(f_pre,cdr g_tm),(cdr o car o concl) th))]
+      val th = REWRITE_RULE [GSYM def_pre] th
+      in (th,def_pre) end  
     val th = UNDISCH_ALL th
-    val rw_th = REWRITE_RULE [GSYM CONJ_ASSOC] (CONJ (SPEC_ALL def) rw_th)
-    in (th,[(t4,func)],i2,rw_th) end
+    val rw_th = CONJ (SPEC_ALL def) (CONJ rw_th1 rw_th2)
+    val rw_pre = CONJ (SPEC_ALL def_pre) (CONJ rw_pre1 rw_pre2)
+    in (th,[(t4,func)],i2,rw_th,rw_pre) end
   else if repeat car instr_tm = ``While`` then let
-    val (th1,lets1,i1,rw_th) = SPEC_FOR_SEQ (cdr instr_tm) (index+1) name rw_th total
+    val (th1,lets1,i1,rw_th1,rw_pre1) = SPEC_FOR_SEQ (cdr instr_tm) (index+1) name total
     val th = MK_SEP_SPEC_WHILE th1 ((cdr o car) instr_tm)
     val (func,p) = (dest_comb o cdr o cdr o concl o UNDISCH_ALL) th
     val f = mk_var(func_name,type_of func)
@@ -265,34 +344,46 @@ fun SPEC_FOR_SEQ instr_tm index name rw_th total = let
     val rw_pre = if not total then TRUTH else let
       val pre_tm = mk_comb(((cdr o concl o SPEC_ALL) def_pre),p)
       val (i,t) = match_term ((cdr o car o concl o SPEC_ALL) PRE_THM) pre_tm
-      val rw_pre = (REWRITE_RULE [GSYM def_pre] o INST i o INST_TYPE t o SPEC_ALL) PRE_THM
+      val rw_pre = (INST i o INST_TYPE t o SPEC_ALL) PRE_THM
+      val rw_pre = PURE_REWRITE_RULE [GSYM def_pre] rw_pre
       val tm = (cdr o cdr o cdr o concl) rw_pre
-      val goal = mk_eq(tm,mk_lets lets1 (mk_comb(car tm,p)))
+      val goal = mk_eq(tm,mk_lets lets1 (mk_comb(car tm, p)))
       val lemma = prove(goal,SIMP_TAC std_ss [LET_DEF] THEN 
                         CONV_TAC (DEPTH_CONV FORCE_PBETA_CONV) THEN SIMP_TAC std_ss [])
       val rw_pre = CONV_RULE ((RAND_CONV o RAND_CONV o RAND_CONV) (fn tm => lemma)) rw_pre
-      in SIMP_RULE std_ss [] rw_pre end
-    val rw_th = REWRITE_RULE [GSYM CONJ_ASSOC] (CONJ (CONJ rw rw_pre) rw_th)
-    in (th,[(p,func_tm)],i1,rw_th) end
+      val rw_pre = SIMP_RULE std_ss [] rw_pre
+      in rw_pre end
+    val rw_th = CONJ (SPEC_ALL rw) rw_th1
+    val rw_pre = CONJ (SPEC_ALL rw_pre) rw_pre1
+    in (th,[(p,func_tm)],i1,rw_th,rw_pre) end
   else raise mk_HOL_ERR "sepOpsemLib" "FUNCTION" 
     ("Program construct not supported: " ^ term_to_string (repeat car instr_tm)) end
 
 fun RAW_SPEC_FOR_CODE instr_tm name total = 
   if mem (repeat car instr_tm) [``While``,``Cond``] then let
-    val (th,lets,_,rw) = SPEC_FOR_SEQ instr_tm 0 name TRUTH total
-    in (th,rw) end 
+    val (th,lets,_,rw,rw_pre) = SPEC_FOR_SEQ instr_tm 0 name total
+    in (th,CONJ rw rw_pre) end 
   else let
-    val (th,lets,_,rw) = SPEC_FOR_SEQ instr_tm 1 name TRUTH total
+    val (th,lets,_,rw,rw_pre) = SPEC_FOR_SEQ instr_tm 1 name total
     val th1 = CONV_RULE (PRE_CONV VARS_UNBETA_CONV THENC POST_CONV VARS_UNBETA_CONV) th
     val p = (cdr o cdr o car o car o concl) th1
     val l1 = mk_lets lets p
     val f = mk_var(name,mk_type("fun",[type_of l1,type_of p]))
     val def = Define [ANTIQUOTE (mk_eq(mk_comb(f,p),l1))]
-    val rw = REWRITE_RULE [GSYM CONJ_ASSOC] (CONJ (SPEC_ALL def) rw)
-    in (th,rw) end;  
+    val rw = CONJ (SPEC_ALL def) rw
+    val f = fst o dest_imp o concl o FORCE_DISCH 
+    val (th,rw_pre) = if f th = T then (th,rw_pre) else let
+      val f_pre = mk_var(name^"_pre",mk_type("fun",[type_of l1,``:bool``]))
+      val def_pre = Define [ANTIQUOTE (mk_eq(mk_comb(f_pre,p),f th))]
+      val rw_pre = CONJ (SPEC_ALL def_pre) rw_pre     
+      val th = CONV_RULE (RATOR_CONV (RAND_CONV (REWRITE_CONV [GSYM def_pre]))) (FORCE_DISCH th)
+      val th = UNDISCH th
+      in (th,rw_pre) end
+    in (th,CONJ rw rw_pre) end;  
 
 fun DERIVE_SEP_SPEC_AUX total name instr_tm = let
   val (th,rw) = RAW_SPEC_FOR_CODE instr_tm name total
+  val rw = REWRITE_RULE [GSYM CONJ_ASSOC] rw
   val f = (fst o dest_eq o concl o hd o CONJUNCTS) rw
   val p = (cdr o cdr o car o car o concl o CONV_RULE (PRE_CONV VARS_UNBETA_CONV)) th
   val q = (cdr o concl) th
@@ -315,13 +406,13 @@ val DERIVE_SEP_SPEC = DERIVE_SEP_SPEC_AUX false;
 val DERIVE_SEP_TOTAL_SPEC = DERIVE_SEP_SPEC_AUX true;
 
 val EXPAND_PAIR_LEMMA = prove(
-  ``!x p q. (x = (p,q)) = (FST x = p) /\ (SND x = q)``,
+  ``!x p q. (x = (p:'a,q:'b)) = (FST x = p) /\ (SND x = q)``,
   Cases THEN SIMP_TAC std_ss []);
 
 fun SEP_SPEC_SEMANTICS th = let
-  val th1 = REWRITE_RULE [SEP_SPEC_def,SPEC_def,LET_DEF] th
+  val th1 = REWRITE_RULE [SEP_SPEC_THM,SEP_TOTAL_SPEC_THM,LET_DEF] (UNDISCH_ALL th)
   val th1 = CONV_RULE (DEPTH_CONV FORCE_PBETA_CONV) th1
-  val th1 = REWRITE_RULE [GSYM STAR_ASSOC,VAR_STAR,FDOM_DOMSUB,IN_DELETE] th1
+  val th1 = REWRITE_RULE [GSYM STAR_ASSOC,VAR_def,ARRAY_def,GEN_VAR_STAR,FDOM_DOMSUB,IN_DELETE] th1
   val th1 = SIMP_RULE std_ss [GSYM AND_IMP_INTRO] th1
   val th1 = REWRITE_RULE [DOMSUB_FAPPLY_THM] th1
   val th1 = SIMP_RULE bool_ss [] th1 
@@ -329,38 +420,15 @@ fun SEP_SPEC_SEMANTICS th = let
   val th1 = REWRITE_RULE [] th1
   val r = genvar(``:state->bool``)
   val s1 = genvar(``:state``)
-  val s2 = genvar(``:state``)
-  val th1 = SPECL [r,s1,s2] th1
-  val tm = (fst o dest_imp o concl o REWRITE_RULE [AND_IMP_INTRO]) th1
+  val th1 = SPECL [r,s1] th1
+  val tm = (cdr o cdr o fst o dest_imp o concl o REWRITE_RULE [AND_IMP_INTRO]) th1
   val v = genvar(``:state``)
-  val frame = mk_abs(v,mk_eq((cdr o cdr o cdr o car) tm,v))
-  val th1 = SIMP_RULE std_ss [] (INST [r|->frame] th1)
-  val vs = all_distinct (find_strings (concl th1))
-  val i = map (fn v => mk_var(fromHOLstring v,``:int``) |-> subst [``s:state``|->s1,``v:string``|->v] 
-                ``(s:state) ' v``) vs
-  val th1 = INST i th1
-  val th1 = INST [s1|->``s1:state``,s2|->``s2:state``] th1
-  val th1 = REWRITE_RULE [] th1     
-  val (a,f) = dest_let (find_term is_let (concl th))
-  val p = fst (dest_pabs a)
-  val s = pred_setSyntax.mk_set (map (fromMLstring o fst o dest_var) (list_dest dest_pair p))
-  val fdom1 = pred_setSyntax.mk_subset(s,``FDOM (s1:state)``)
-  val fdom2 = subst [``s1:state``|->``s2:state``] fdom1 
-  val vs = map (fst o dest_var) (find_terms is_var f)
-  val i = map (fn v => mk_var(v,``:int``) |-> (subst [``s:string``|->fromMLstring v] ``s1:state ' s``)) vs
-  val f = subst i f
-  val p = subst [``s1:state``|->``s2:state``] (subst i p)
-  val tm = mk_eq(f,p)
-  val (x,y) = (dest_imp o concl o REWRITE_RULE [AND_IMP_INTRO,CONJ_ASSOC]) th1
-  val goal = mk_imp(mk_conj(fdom1,cdr x),mk_conj(tm,mk_conj(fdom2,cdr y)))
-  val goal = mk_forall(``s1:state``,mk_forall(``s2:state``,goal))
-  val result = prove(goal,
-    REWRITE_TAC [INSERT_SUBSET,EMPTY_SUBSET,EXPAND_PAIR_LEMMA] THEN REPEAT STRIP_TAC   
-    THEN STRIP_ASSUME_TAC (UNDISCH_ALL th1) THEN ASM_REWRITE_TAC [])
-  in result end;
-
-fun DERIVE_FUNCTION name term = let
-  val (th,rw) = DERIVE_SEP_SPEC name term
-  in (th,SEP_SPEC_SEMANTICS th, rw) end;
+  val frame = mk_abs(v,mk_eq(tm,v))
+  val th1 = INST [r|->frame] th1
+  val th1 = INST [s1|->``s1:state``] th1
+  val th1 = SIMP_RULE std_ss [AND_IMP_INTRO,GSYM CONJ_ASSOC] (DISCH_ALL th1)
+  val th1 = GEN ``s1:state`` th1 
+  in th1 end;
+  
 
 end
